@prefix owl: <http://www.w3.org/2002/07/owl#> .
@prefix rdfs: <http://www.w3.org/2000/01/rdf-schema#> .
@prefix xsd: <http://www.w3.org/2001/XMLSchema#> .
@prefix dct: <http://purl.org/dc/terms/> .
@prefix peco: <https://w3id.org/peco#> .
@prefix foaf: <http://xmlns.com/foaf/0.1/> .
@prefix cto: <https://example.org/cto#> .

<https://example.org/cto>
    a owl:Ontology ;
    rdfs:label "Carbon Trade Ontology (extension of PECO)" ;
    rdfs:comment "Extension of PECO to represent carbon credits and trading." ;
    dct:creator "AlisaInari" ;
    dct:created "2025-07-25"^^xsd:date ;
    owl:imports <https://w3id.org/peco> .

#Add how credit calculated or where it comes from (peco:EmissionScore), also what activity the sequestration comes from?
#classes

cto:CarbonCredit a owl:Class ;
    rdfs:label "Carbon Credit" ;
    rdfs:subClassOf peco:EmissionsResult ;
    rdfs:comment "A unit representing a verified reduction or removal of carbon dioxide equivalent (CO₂e)." .

#object properties

cto:issuedBy a owl:ObjectProperty ;
    rdfs:domain cto:CarbonCredit ;
    rdfs:range foaf:Organization ;
    rdfs:label "issued by" ;
    rdfs:comment "Relation linking a carbon credit to the organization that issued it." .

cto:registeredIn a owl:ObjectProperty ;
    rdfs:domain cto:CarbonCredit ;
    rdfs:range rdfs:Resource ;
    rdfs:label "registered in" ;
    rdfs:comment "A registry or platform in which the carbon credit is listed." .

#datatype (or should just use qudt:quantity with qudt:unit?)

cto:creditAmount a owl:DatatypeProperty ;
    rdfs:domain cto:CarbonCredit ;
    rdfs:range xsd:decimal ;
    rdfs:label "credit amount" ;
    rdfs:comment "The amount of CO₂e (in tonnes) represented by the credit." .



